- Fixed the fixpoint combinator semantics and type - Introduced labelled transitions and labels for computation placeholders - Now the double computation fork death reduces based on the select operator (they could be in two orders we may not pick one as that would break commutativity). Note how there is a specificity order of reduction for this case, so that we end up returning { unit, unit } rather than {unit, live exp unit } though this seems not mandatory.

mconbase.v
@@ -11,6 +11,12 @@ Proof.
   decide equality; auto with ott_coq_equality arith.
 Defined.
 Hint Resolve eq_value_name : ott_coq_equality.
+Definition label := nat.
+Lemma eq_label: forall (x y : label), {x = y} + {x <> y}.
+Proof.
+  decide equality; auto with ott_coq_equality arith.
+Defined.
+Hint Resolve eq_label : ott_coq_equality.
 Definition ident := nat.
 Definition index := nat.
 
@@ -34,12 +40,16 @@ Inductive constant : Set :=
  | CONST_unit : constant
  | CONST_stop : constant.
 
+Inductive redlabel : Set := 
+ | RL_tau : redlabel
+ | RL_labelled (lab:label).
+
 Inductive list_typvar : Set := 
  | Nil_list_typvar : list_typvar
  | Cons_list_typvar (_:typvar) (_:list_typvar).
 
 Inductive livemodes : Set := 
- | LM_comp : livemodes
+ | LM_comp (rl:redlabel)
  | LM_expr (expr5:expr)
 with expr : Set := 
  | E_ident (value_name5:value_name)
@@ -159,32 +169,6 @@ Definition tsubst_typscheme (sub:list (typvar*typexpr)) (ts5:typscheme) : typsch
   | (TS_ts typvar_list typexpr5) => TS_ts typvar_list (tsubst_typexpr (list_minus2 eq_typvar sub (unmake_list_typvar typvar_list)) typexpr5)
 end.
 
-Fixpoint tsubst_expr (sub:list (typvar*typexpr)) (e_5:expr) {struct e_5} : expr :=
-  match e_5 with
-  | (E_ident value_name5) => E_ident value_name5
-  | (E_constant constant5) => E_constant constant5
-  | (E_apply expr5 expr') => E_apply (tsubst_expr sub expr5) (tsubst_expr sub expr')
-  | (E_bind expr5 expr') => E_bind (tsubst_expr sub expr5) (tsubst_expr sub expr')
-  | (E_function value_name5 typexpr5 expr5) => E_function value_name5 (tsubst_typexpr sub typexpr5) (tsubst_expr sub expr5)
-  | (E_fix e) => E_fix (tsubst_expr sub e)
-  | (E_live_expr lm) => E_live_expr (tsubst_livemodes sub lm)
-  | (E_pair e e') => E_pair (tsubst_expr sub e) (tsubst_expr sub e')
-  | (E_taggingleft e) => E_taggingleft (tsubst_expr sub e)
-  | (E_taggingright e) => E_taggingright (tsubst_expr sub e)
-  | (E_case e1 x1 e2 x2 e3) => E_case (tsubst_expr sub e1) x1 (tsubst_expr sub e2) x2 (tsubst_expr sub e3)
-end
-with tsubst_livemodes (sub:list (typvar*typexpr)) (lm5:livemodes) {struct lm5} : livemodes :=
-  match lm5 with
-  | LM_comp => LM_comp 
-  | (LM_expr expr5) => LM_expr (tsubst_expr sub expr5)
-end.
-
-Fixpoint tsubst_G (sub:list (typvar*typexpr)) (G_6:G) {struct G_6} : G :=
-  match G_6 with
-  | G_em => G_em 
-  | (G_vn G5 value_name5 typscheme5) => G_vn (tsubst_G sub G5) value_name5 (tsubst_typscheme sub typscheme5)
-end.
-
 Fixpoint subst_expr (e_5:expr) (x_5:value_name) (e__6:expr) {struct e__6} : expr :=
   match e__6 with
   | (E_ident value_name5) => (if eq_value_name value_name5 x_5 then e_5 else (E_ident value_name5))
@@ -201,8 +185,34 @@ Fixpoint subst_expr (e_5:expr) (x_5:value_name) (e__6:expr) {struct e__6} : expr
 end
 with subst_livemodes (e5:expr) (x5:value_name) (lm5:livemodes) {struct lm5} : livemodes :=
   match lm5 with
-  | LM_comp => LM_comp 
+  | (LM_comp rl) => LM_comp rl
   | (LM_expr expr5) => LM_expr (subst_expr e5 x5 expr5)
+end.
+
+Fixpoint tsubst_expr (sub:list (typvar*typexpr)) (e_5:expr) {struct e_5} : expr :=
+  match e_5 with
+  | (E_ident value_name5) => E_ident value_name5
+  | (E_constant constant5) => E_constant constant5
+  | (E_apply expr5 expr') => E_apply (tsubst_expr sub expr5) (tsubst_expr sub expr')
+  | (E_bind expr5 expr') => E_bind (tsubst_expr sub expr5) (tsubst_expr sub expr')
+  | (E_function value_name5 typexpr5 expr5) => E_function value_name5 (tsubst_typexpr sub typexpr5) (tsubst_expr sub expr5)
+  | (E_fix e) => E_fix (tsubst_expr sub e)
+  | (E_live_expr lm) => E_live_expr (tsubst_livemodes sub lm)
+  | (E_pair e e') => E_pair (tsubst_expr sub e) (tsubst_expr sub e')
+  | (E_taggingleft e) => E_taggingleft (tsubst_expr sub e)
+  | (E_taggingright e) => E_taggingright (tsubst_expr sub e)
+  | (E_case e1 x1 e2 x2 e3) => E_case (tsubst_expr sub e1) x1 (tsubst_expr sub e2) x2 (tsubst_expr sub e3)
+end
+with tsubst_livemodes (sub:list (typvar*typexpr)) (lm5:livemodes) {struct lm5} : livemodes :=
+  match lm5 with
+  | (LM_comp rl) => LM_comp rl
+  | (LM_expr expr5) => LM_expr (tsubst_expr sub expr5)
+end.
+
+Fixpoint tsubst_G (sub:list (typvar*typexpr)) (G_6:G) {struct G_6} : G :=
+  match G_6 with
+  | G_em => G_em 
+  | (G_vn G5 value_name5 typscheme5) => G_vn (tsubst_G sub G5) value_name5 (tsubst_typscheme sub typscheme5)
 end.
 
 (** library functions *)
@@ -246,7 +256,7 @@ Fixpoint ftv_expr (e_5:expr) : list typvar :=
 end
 with ftv_livemodes (lm5:livemodes) : list typvar :=
   match lm5 with
-  | LM_comp => nil
+  | (LM_comp rl) => nil
   | (LM_expr expr5) => ((ftv_expr expr5))
 end.
 
@@ -306,11 +316,11 @@ with Get : G -> expr -> typexpr -> Prop :=    (* defn Get *)
  | Get_live_exp : forall (G5:G) (e:expr) (t:typexpr),
      Get G5 e t ->
      Get G5 (E_live_expr (LM_expr e)) (TE_concurrent t)
- | Get_live_comp : forall (G5:G),
-     Get G5 (E_live_expr LM_comp) (TE_concurrent (TE_constants TC_unit))
- | Get_fix : forall (G5:G) (e:expr) (t:typexpr),
-     Get G5 e (TE_arrow t t) ->
-     Get G5 (E_fix e) t
+ | Get_live_comp : forall (G5:G) (rl:redlabel),
+     Get G5 (E_live_expr  (LM_comp rl) ) (TE_concurrent (TE_constants TC_unit))
+ | Get_fix : forall (G5:G) (e:expr) (t t':typexpr),
+     Get G5 e (TE_arrow  (TE_arrow t t')   (TE_arrow t t') ) ->
+     Get G5 (E_fix e)  (TE_arrow t t') 
  | Get_bind : forall (G5:G) (e e':expr) (t' t:typexpr),
      Get G5 e (TE_concurrent t) ->
      Get G5 e' (TE_arrow t (TE_concurrent t')) ->
@@ -333,83 +343,89 @@ with Get : G -> expr -> typexpr -> Prop :=    (* defn Get *)
 (** definitions *)
 
 (* defns Jop *)
-Inductive JO_red : expr -> select -> expr -> Prop :=    (* defn red *)
+Inductive JO_red : expr -> select -> redlabel -> expr -> Prop :=    (* defn red *)
  | JO_red_app : forall (x:value_name) (t:typexpr) (e:expr) (s:select) (v:expr),
      is_value_of_expr v ->
-     JO_red (E_apply  (E_function x t e)  v) s  (subst_expr  v   x   e ) 
- | JO_red_forkmove1 : forall (e e' e'':expr) (s:select),
+     JO_red (E_apply  (E_function x t e)  v) s RL_tau  (subst_expr  v   x   e ) 
+ | JO_red_forkmove1 : forall (e e':expr) (rl:redlabel) (e'':expr) (s:select),
      ~ ( is_value_of_expr ( e' ) )  ->
-     JO_red e s e'' ->
-     JO_red (E_apply  (E_apply (E_constant CONST_fork)  (E_live_expr (LM_expr e)) )   (E_live_expr (LM_expr e')) ) S_First (E_apply  (E_apply (E_constant CONST_fork)  (E_live_expr (LM_expr e'')) )   (E_live_expr (LM_expr e')) )
- | JO_red_forkmove2 : forall (e e' e'':expr) (s:select),
+     JO_red e s rl e'' ->
+     JO_red (E_apply  (E_apply (E_constant CONST_fork)  (E_live_expr (LM_expr e)) )   (E_live_expr (LM_expr e')) ) S_First rl (E_apply  (E_apply (E_constant CONST_fork)  (E_live_expr (LM_expr e'')) )   (E_live_expr (LM_expr e')) )
+ | JO_red_forkmove2 : forall (e e':expr) (rl:redlabel) (e'':expr) (s:select),
      ~ ( is_value_of_expr ( e ) )  ->
-     JO_red e' s e'' ->
-     JO_red (E_apply  (E_apply (E_constant CONST_fork)  (E_live_expr (LM_expr e)) )   (E_live_expr (LM_expr e')) ) S_Second (E_apply  (E_apply (E_constant CONST_fork)  (E_live_expr (LM_expr e)) )   (E_live_expr (LM_expr e'')) )
+     JO_red e' s rl e'' ->
+     JO_red (E_apply  (E_apply (E_constant CONST_fork)  (E_live_expr (LM_expr e)) )   (E_live_expr (LM_expr e')) ) S_Second rl (E_apply  (E_apply (E_constant CONST_fork)  (E_live_expr (LM_expr e)) )   (E_live_expr (LM_expr e'')) )
  | JO_red_forkdeath1 : forall (v e:expr) (s:select),
      is_value_of_expr v ->
-     JO_red (E_apply  (E_apply (E_constant CONST_fork)  (E_live_expr (LM_expr v)) )   (E_live_expr (LM_expr e)) ) s (E_live_expr (LM_expr  (E_taggingleft  (E_taggingright  (E_pair v  (E_live_expr (LM_expr e)) ) ) ) ))
+     JO_red (E_apply  (E_apply (E_constant CONST_fork)  (E_live_expr (LM_expr v)) )   (E_live_expr (LM_expr e)) ) s RL_tau (E_live_expr (LM_expr  (E_taggingleft  (E_taggingright  (E_pair v  (E_live_expr (LM_expr e)) ) ) ) ))
  | JO_red_forkdeath2 : forall (e v':expr) (s:select),
      is_value_of_expr v' ->
-     JO_red (E_apply  (E_apply (E_constant CONST_fork)  (E_live_expr (LM_expr e)) )   (E_live_expr (LM_expr v')) ) s (E_live_expr (LM_expr  (E_taggingright  (E_pair  (E_live_expr (LM_expr e))  v') ) ))
+     JO_red (E_apply  (E_apply (E_constant CONST_fork)  (E_live_expr (LM_expr e)) )   (E_live_expr (LM_expr v')) ) s RL_tau (E_live_expr (LM_expr  (E_taggingright  (E_pair  (E_live_expr (LM_expr e))  v') ) ))
  | JO_red_forkdeath12 : forall (v v':expr) (s:select),
      is_value_of_expr v ->
      is_value_of_expr v' ->
-     JO_red (E_apply  (E_apply (E_constant CONST_fork)  (E_live_expr (LM_expr v)) )   (E_live_expr (LM_expr v')) ) s (E_live_expr (LM_expr  (E_taggingleft  (E_taggingleft  (E_pair v v') ) ) ))
- | JO_red_forkdocomp1 : forall (e:expr) (s:select),
-     JO_red (E_apply  (E_apply (E_constant CONST_fork)  (E_live_expr LM_comp) )   (E_live_expr (LM_expr e)) ) s (E_live_expr (LM_expr  (E_taggingleft  (E_taggingright  (E_pair (E_constant CONST_unit)  (E_live_expr (LM_expr e)) ) ) ) ))
- | JO_red_forkdocomp2 : forall (e:expr) (s:select),
-     JO_red (E_apply  (E_apply (E_constant CONST_fork)  (E_live_expr (LM_expr e)) )   (E_live_expr LM_comp) ) s (E_live_expr (LM_expr  (E_taggingright  (E_pair  (E_live_expr (LM_expr e))  (E_constant CONST_unit)) ) ))
- | JO_red_forkdocomp12 : forall (s:select),
-     JO_red (E_apply  (E_apply (E_constant CONST_fork)  (E_live_expr LM_comp) )   (E_live_expr LM_comp) ) s (E_live_expr (LM_expr  (E_taggingleft  (E_taggingleft  (E_pair (E_constant CONST_unit) (E_constant CONST_unit)) ) ) ))
+     JO_red (E_apply  (E_apply (E_constant CONST_fork)  (E_live_expr (LM_expr v)) )   (E_live_expr (LM_expr v')) ) s RL_tau (E_live_expr (LM_expr  (E_taggingleft  (E_taggingleft  (E_pair v v') ) ) ))
+ | JO_red_forkdocomp1 : forall (rl:redlabel) (e:expr) (s:select),
+     JO_red (E_apply  (E_apply (E_constant CONST_fork)  (E_live_expr  (LM_comp rl) ) )   (E_live_expr (LM_expr e)) ) s rl (E_live_expr (LM_expr  (E_taggingleft  (E_taggingright  (E_pair (E_constant CONST_unit)  (E_live_expr (LM_expr e)) ) ) ) ))
+ | JO_red_forkdocomp2 : forall (e:expr) (rl:redlabel) (s:select),
+     JO_red (E_apply  (E_apply (E_constant CONST_fork)  (E_live_expr (LM_expr e)) )   (E_live_expr  (LM_comp rl) ) ) s rl (E_live_expr (LM_expr  (E_taggingright  (E_pair  (E_live_expr (LM_expr e))  (E_constant CONST_unit)) ) ))
+ | JO_red_forkdocomp12 : forall (rl rl':redlabel),
+     JO_red (E_apply  (E_apply (E_constant CONST_fork)  (E_live_expr  (LM_comp rl) ) )   (E_live_expr  (LM_comp rl') ) ) S_First rl (E_apply  (E_apply (E_constant CONST_fork)  (E_live_expr  (LM_expr (E_constant CONST_unit)) ) )   (E_live_expr  (LM_comp rl') ) )
+ | JO_red_forkdocomp21 : forall (rl rl':redlabel),
+     JO_red (E_apply  (E_apply (E_constant CONST_fork)  (E_live_expr  (LM_comp rl) ) )   (E_live_expr  (LM_comp rl') ) ) S_Second rl' (E_apply  (E_apply (E_constant CONST_fork)  (E_live_expr  (LM_comp rl) ) )   (E_live_expr  (LM_expr (E_constant CONST_unit)) ) )
+ | JO_red_forkfincomp12 : forall (rl':redlabel) (s:select),
+     JO_red (E_apply  (E_apply (E_constant CONST_fork)  (E_live_expr  (LM_expr (E_constant CONST_unit)) ) )   (E_live_expr  (LM_comp rl') ) ) s rl' (E_live_expr (LM_expr  (E_taggingleft  (E_taggingleft  (E_pair (E_constant CONST_unit) (E_constant CONST_unit)) ) ) ))
+ | JO_red_forkfincomp21 : forall (rl:redlabel) (s:select),
+     JO_red (E_apply  (E_apply (E_constant CONST_fork)  (E_live_expr  (LM_comp rl) ) )   (E_live_expr  (LM_expr (E_constant CONST_unit)) ) ) s rl (E_live_expr (LM_expr  (E_taggingleft  (E_taggingleft  (E_pair (E_constant CONST_unit) (E_constant CONST_unit)) ) ) ))
  | JO_red_ret : forall (v:expr) (s:select),
      is_value_of_expr v ->
-     JO_red (E_apply (E_constant CONST_ret) v) s  (E_live_expr (LM_expr v)) 
- | JO_red_evalbind : forall (e e'':expr) (s:select) (e':expr),
-     JO_red e s e' ->
-     JO_red (E_bind e e'') s (E_bind e' e'')
- | JO_red_movebind : forall (e e'':expr) (s:select) (e':expr),
-     JO_red e s e' ->
-     JO_red (E_bind  (E_live_expr (LM_expr e))  e'') s (E_bind  (E_live_expr (LM_expr e'))  e'')
- | JO_red_compbind : forall (e:expr) (s:select) (e':expr),
-     JO_red (E_bind  (E_live_expr LM_comp)  e) s (E_apply e' (E_constant CONST_unit))
+     JO_red (E_apply (E_constant CONST_ret) v) s RL_tau  (E_live_expr (LM_expr v)) 
+ | JO_red_evalbind : forall (e e'':expr) (s:select) (rl:redlabel) (e':expr),
+     JO_red e s rl e' ->
+     JO_red (E_bind e e'') s rl (E_bind e' e'')
+ | JO_red_movebind : forall (e e'':expr) (s:select) (rl:redlabel) (e':expr),
+     JO_red e s rl e' ->
+     JO_red (E_bind  (E_live_expr (LM_expr e))  e'') s rl (E_bind  (E_live_expr (LM_expr e'))  e'')
+ | JO_red_compbind : forall (rl:redlabel) (e:expr) (s:select) (e':expr),
+     JO_red (E_bind  (E_live_expr  (LM_comp rl) )  e) s rl (E_apply e' (E_constant CONST_unit))
  | JO_red_dobind : forall (v e:expr) (s:select),
      is_value_of_expr v ->
-     JO_red (E_bind  (E_live_expr (LM_expr v))  e) s (E_apply e v)
- | JO_red_context_app1 : forall (e e':expr) (s:select) (e'':expr),
-     JO_red e' s e'' ->
-     JO_red (E_apply e e') s (E_apply e e'')
- | JO_red_context_app2 : forall (e v:expr) (s:select) (e':expr),
+     JO_red (E_bind  (E_live_expr (LM_expr v))  e) s RL_tau (E_apply e v)
+ | JO_red_context_app1 : forall (e e':expr) (s:select) (rl:redlabel) (e'':expr),
+     JO_red e' s rl e'' ->
+     JO_red (E_apply e e') s rl (E_apply e e'')
+ | JO_red_context_app2 : forall (e v:expr) (s:select) (rl:redlabel) (e':expr),
      is_value_of_expr v ->
-     JO_red e s e' ->
-     JO_red (E_apply e v) s (E_apply e' v)
- | JO_red_fix_move : forall (e:expr) (s:select) (e':expr),
-     JO_red e s e' ->
-     JO_red  (E_fix e)  s  (E_fix e') 
+     JO_red e s rl e' ->
+     JO_red (E_apply e v) s rl (E_apply e' v)
+ | JO_red_fix_move : forall (e:expr) (s:select) (rl:redlabel) (e':expr),
+     JO_red e s rl e' ->
+     JO_red  (E_fix e)  s rl  (E_fix e') 
  | JO_red_fix_app : forall (v v':expr) (s:select),
      is_value_of_expr v ->
      is_value_of_expr v' ->
-     JO_red (E_apply  (E_fix v)  v') s (E_apply  (E_fix v)   (E_apply v v') )
- | JO_red_pair_1 : forall (e e'':expr) (s:select) (e':expr),
-     JO_red e s e' ->
-     JO_red (E_pair e e'') s (E_pair e' e'')
- | JO_red_pair_2 : forall (v e:expr) (s:select) (e':expr),
+     JO_red (E_apply  (E_fix v)  v') s RL_tau (E_apply  (E_apply v  (E_fix v) )   v' )
+ | JO_red_pair_1 : forall (e e'':expr) (s:select) (rl:redlabel) (e':expr),
+     JO_red e s rl e' ->
+     JO_red (E_pair e e'') s rl (E_pair e' e'')
+ | JO_red_pair_2 : forall (v e:expr) (s:select) (rl:redlabel) (e':expr),
      is_value_of_expr v ->
-     JO_red e s e' ->
-     JO_red (E_pair v e) s (E_pair v e')
- | JO_red_evalinl : forall (e:expr) (s:select) (e':expr),
-     JO_red e s e' ->
-     JO_red (E_taggingleft e) s (E_taggingleft e')
- | JO_red_evalinr : forall (e:expr) (s:select) (e':expr),
-     JO_red e s e' ->
-     JO_red (E_taggingright e) s (E_taggingright e')
+     JO_red e s rl e' ->
+     JO_red (E_pair v e) s rl (E_pair v e')
+ | JO_red_evalinl : forall (e:expr) (s:select) (rl:redlabel) (e':expr),
+     JO_red e s rl e' ->
+     JO_red (E_taggingleft e) s rl (E_taggingleft e')
+ | JO_red_evalinr : forall (e:expr) (s:select) (rl:redlabel) (e':expr),
+     JO_red e s rl e' ->
+     JO_red (E_taggingright e) s rl (E_taggingright e')
  | JO_red_evalcaseinl : forall (x:value_name) (e:expr) (x':value_name) (e':expr) (s:select) (v:expr),
      is_value_of_expr v ->
-     JO_red (E_case  (E_taggingleft v)  x e x' e') s  (subst_expr  v   x   e ) 
+     JO_red (E_case  (E_taggingleft v)  x e x' e') s RL_tau  (subst_expr  v   x   e ) 
  | JO_red_evalcaseinr : forall (x:value_name) (e:expr) (x':value_name) (e':expr) (s:select) (v:expr),
      is_value_of_expr v ->
-     JO_red (E_case  (E_taggingright v)  x e x' e') s  (subst_expr  v   x'   e' ) 
- | JO_red_evalcase : forall (e:expr) (x:value_name) (e'':expr) (x':value_name) (e''':expr) (s:select) (e':expr),
-     JO_red e s e' ->
-     JO_red (E_case e x e'' x' e''') s (E_case e' x e'' x' e''').
+     JO_red (E_case  (E_taggingright v)  x e x' e') s RL_tau  (subst_expr  v   x'   e' ) 
+ | JO_red_evalcase : forall (e:expr) (x:value_name) (e'':expr) (x':value_name) (e''':expr) (s:select) (rl:redlabel) (e':expr),
+     JO_red e s rl e' ->
+     JO_red (E_case e x e'' x' e''') s rl (E_case e' x e'' x' e''').
 
 
